theories/misc.v
@@ -1,0 +1,123 @@
+(******************************************************************************)
+(*                                                                            *)
+(*                                  Marble                                    *)
+(*                                                                            *)
+(*                       François Pottier, Inria Paris                        *)
+(*                                                                            *)
+(*       Copyright 2026--2026 Inria. All rights reserved. This file is        *)
+(*       distributed under the terms of the GNU Library General Public        *)
+(*       License, with an exception, as described in the file LICENSE.        *)
+(*                                                                            *)
+(******************************************************************************)
+
+From stdpp Require Import numbers list.
+From stdpp Require Import sets propset.
+From listz Require Import listz.
+From marble.logic Require Import sets.
+Notation len := length.
+From marble Require Import tactics bool int wp iteration.
+
+(* We prove that the specifications [ITER_SET] and [ITER_SET'] are
+   equivalent. *)
+
+Section Equivalence.
+
+Context {S A : Type} `{SemiSet A C}.
+
+Variable (body : A → S → WP S).
+Variable (loop : S → WP S).
+
+(* We must assume that [body] and [loop] are covariant; that is,
+   they support the consequence rule. These assumptions mean that
+   this equivalence proof may be a little inconvenient to use in
+   practice. *)
+
+Variable body_covariant :
+  ∀ x s Q Q',
+  body x s Q →
+  (∀ s, Q s → Q' s) →
+  body x s Q'.
+
+Variable loop_covariant :
+  ∀ s Q Q',
+  loop s Q →
+  (∀ s, Q s → Q' s) →
+  loop s Q'.
+
+Lemma direction1 (init xs : C) (init' : list A) :
+  ITER_SET init xs body loop →
+  list_to_set init' ≡ init →
+  ITER_SET' init' xs body loop.
+Proof.
+  intros Hspec Hseed. ITER.
+  eapply loop_covariant.
+  { eapply Hspec with (inv :=
+      λ xs s, ∃ history,
+        inv history s ∧
+        init' `prefix_of` history ∧
+        list_to_set history ≡ xs
+    ); clear Hspec.
+    (* Compatibility. *)
+    { clear dependent s.
+      intros xs1 xs2 Hequiv. intros s ? <-.
+      split; intros; unpack; pack; eauto.
+      + rewrite <- Hequiv. eauto.
+      + rewrite Hequiv. eauto. }
+    (* Initialization. *)
+    { pack; eauto. }
+    (* Preservation. *)
+    { clear dependent s.
+      intros j0 j1 s (history0 & ? & ? & ?).
+      intros x ???.
+      eapply body_covariant.
+      { eauto with set_solver. }
+      cbv beta. pack; eauto using prefix_app_r. set_solver. }
+    }
+  cbv beta. clear Hspec Hbody. clear dependent s.
+  intros s (xs' & Hpost).
+  destruct Hpost as ((history & ? & ? & ?) & ?).
+  pack; eauto. set_solver.
+Qed.
+
+Lemma list_to_set_prefix_of (xs ys : list A) :
+  xs `prefix_of` ys →
+  list_to_set xs ⊆ (list_to_set ys : C).
+Proof.
+  intros. intro x. set_unfold. eauto using elem_of_prefix.
+Qed.
+
+Lemma direction2 (init xs : C) (init' : list A) :
+  ITER_SET' init' xs body loop →
+  list_to_set init' ≡ init →
+  ITER_SET init xs body loop.
+Proof.
+  intros Hspec Hseed. ITER.
+  eapply loop_covariant.
+  { eapply Hspec with (inv := λ history s, inv (list_to_set history) s);
+    clear Hspec.
+    (* Compatibility. *)
+    { clear Hbody. clear dependent s.
+      intros history1 history2 Hequiv.
+      unfold equiv in Hequiv. subst history2.
+      intros s ? <-.
+      split; intros; unpack; pack; eauto. }
+    (* Initialization. *)
+    { set_solver. }
+    (* Preservation. *)
+    { clear dependent s.
+      intros j0 j1 s ?. intros x ???.
+      eapply body_covariant.
+      { eapply Hbody; eauto.
+        + rewrite <- Hseed.
+          eauto using list_to_set_prefix_of.
+        + set_solver. }
+      cbv beta. subst j1. pack.
+      rewrite list_to_set_app, list_to_set_singleton. assumption. }
+  }
+  cbv beta. clear Hspec Hbody. clear dependent s.
+  intros s (history & Hpost).
+  destruct Hpost.
+  pack; eauto with set_solver.
+Qed.
+
+End Equivalence.
